Tealeaves/Examples/STLC/TypeSoundness.v
@@ -2,27 +2,39 @@ From Tealeaves Require Export
   Examples.STLC.Syntax
   Examples.STLC.Simplification.
 
+Export LN.Notations.
 Export STLC.Syntax.Notations.
 #[local] Open Scope set_scope.
 
+Implicit Types (x: atom) (τ: typ)
+  (t u: term LN) (n: nat) (v: LN) (Γ : ctx).
+
+Ltac gather_atoms ::=
+  let A := gather_atoms_with (fun s : AtomSet.t => s) in
+  let B := gather_atoms_with (fun x : atom => {{ x }}) in
+  let C := gather_atoms_with (fun t : term LN => FV t) in
+  let D := gather_atoms_with (fun Γ : alist typ => domset Γ) in
+  constr:(A ∪ B ∪ C ∪ D).
+
 (** * Inversion lemmas *)
 (******************************************************************************)
-Lemma inversion11 : forall (A : typ) (x : atom) (Γ : ctx),
-    Γ ⊢ tvar (Fr x) : A -> (x, A) ∈ Γ.
+Lemma inversion11 : forall (τ: typ) (x : atom) (Γ : ctx),
+    Γ ⊢ tvar (Fr x) : τ -> (x, τ) ∈ Γ.
 Proof.
   inversion 1; auto.
 Qed.
 
-Lemma inversion12 : forall (A : typ) (n : nat) (Γ : ctx),
-    Γ ⊢ tvar (Bd n) : A -> False.
+Lemma inversion12 : forall (τ: typ) (n : nat) (Γ : ctx),
+    Γ ⊢ tvar (Bd n) : τ -> False.
 Proof.
   inversion 1; auto.
 Qed.
 
 (* This is somewhat weak because L should really be (dom Γ) *)
-Lemma inversion21 : forall (A B : typ) (e : term LN) (Γ : ctx),
-    (Γ ⊢ λ A e : B) ->
-    exists C, B = A ⟹ C /\ exists L, forall (x : atom), ~ AtomSet.In x L -> Γ ++ x ~ A ⊢ e '(tvar (Fr x)) : C.
+Lemma inversion21 : forall (τ B : typ) (e : term LN) (Γ : ctx),
+    (Γ ⊢ λ τ e : B) ->
+    exists C, B = τ ⟹ C /\ exists L, forall (x : atom),
+        x `notin` L -> Γ ++ x ~ τ ⊢ e '(tvar (Fr x)) : C.
 Proof.
   introv J.
   inversion J; subst.
@@ -30,161 +42,162 @@ Proof.
 Qed.
 
 (** Inversion principle for [abs] where we may assume the abstraction has arrow type *)
-Lemma inversion22 : forall (A B : typ) (e : term LN) (Γ : ctx),
-    (Γ ⊢ λ A e : A ⟹ B) ->
-    exists L, forall (x : atom), ~ AtomSet.In x L -> Γ ++ x ~ A ⊢ e '(tvar (Fr x)) : B.
+Lemma inversion22 : forall (τ τ' : typ) (e : term LN) (Γ : ctx),
+    Γ ⊢ λ τ e : τ ⟹ τ' ->
+    exists L, forall (x : atom),
+      x `notin` L ->
+      Γ ++ x ~ τ ⊢ e '(x: term LN) : τ'.
 Proof.
   introv J. apply inversion21 in J.
   destruct J as [C [H1 H2]].
-  assert (B = C) by (inversion H1; auto); subst.
+  assert (τ' = C) by (inversion H1; auto); subst.
   assumption.
 Qed.
 
-Lemma inversion3 : forall (A : typ) (Γ : ctx) (t1 t2 : term LN),
-    (Γ ⊢ [t1]@[t2] : A) ->
-    exists B, (Γ ⊢ t1 : B ⟹ A) /\ (Γ ⊢ t2 : B).
+Lemma inversion3 : forall (τ: typ) (Γ : ctx) (t1 t2 : term LN),
+    (Γ ⊢ ⟨t1⟩ (t2) : τ) ->
+    exists τ', (Γ ⊢ t1 : τ' ⟹ τ)
+          /\ (Γ ⊢ t2 : τ').
 Proof.
-  introv J; inversion J; subst.
-  exists A0. split; auto.
+  introv J; inversion J; subst; eauto.
 Qed.
 
 (** * Misc lemmas *)
 (******************************************************************************)
-Theorem j_ctx_wf : forall Γ (t : term LN) (A : typ),
-    Γ ⊢ t : A -> uniq Γ.
+Theorem j_ctx_wf : forall Γ (t : term LN) (τ: typ),
+    Γ ⊢ t : τ -> uniq Γ.
 Proof.
-  introv J. induction J.
+  introv J; typing_induction.
   - assumption.
-  - specialize_freshly H0.
-    now autorewrite with tea_rw_uniq in H0.
+  - specialize_freshly IHbody.
+    now autorewrite with tea_rw_uniq in IHbody.
   - assumption.
 Qed.
 
-Ltac gather_atoms ::=
-  let A := gather_atoms_with (fun s : AtomSet.t => s) in
-  let B := gather_atoms_with (fun x : atom => {{ x }}) in
-  let C := gather_atoms_with (fun t : term LN => freeset t) in
-  let D := gather_atoms_with (fun Γ : alist typ => domset Γ) in
-  constr:(A ∪ B ∪ C ∪ D).
-
-Theorem j_wf : forall Γ (t : term LN) (A : typ),
-    Γ ⊢ t : A -> scoped t (domset Γ).
+Theorem j_wf : forall Γ (t : term LN) (τ: typ),
+    Γ ⊢ t : τ -> FV t ⊆ domset Γ.
 Proof.
-  introv J. induction J.
-  - rename H0 into Hin.
-    unfold scoped.
-    rewrite term_freeset12.
+  introv J. typing_induction.
+  - simplify.
     apply in_in_domset in Hin.
     fsetdec.
-  - rename H0 into IH; rename H into premise.
-    specialize_freshly IH.
-    unfold scoped in *.
-    rewrite term_freeset2.
-    assert (step1 : freeset t ⊆ freeset (t '(tvar (Fr e))))
-      by apply freeset_open_lower.
-    assert (step2 : forall x, x ∈@ (freeset t) -> x ∈@ (domset (Γ ++ e ~ τ1)))
+  - specialize_freshly IHbody.
+    simplify.
+    assert (step1 : FV body ⊆ FV (body '(e: term LN)))
+      by apply FV_open_lower.
+    assert (step2 : forall x, x `in` FV body -> x `in` (domset (Γ ++ e ~ τ1)))
       by fsetdec.
-    intros x xin. assert (x <> e) by fsetdec.
+    intros x xin.
+    assert (x <> e) by fsetdec.
     specialize (step2 x xin).
     rewrite domset_app in step2.
-    cbn in step2. fsetdec.
-  - unfold scoped in *.
-    rewrite term_freeset3.
+    rewrite domset_one in step2.
     fsetdec.
-Qed.
-
-Theorem is_bound_or_free_monotone : forall (k w1 w2 : nat) (l : LN),
-    w1 < w2 ->
-    is_bound_or_free k (w1, l) ->
-    is_bound_or_free k (w2, l).
-Proof.
-  cbn. unfold_ops @Monoid_op_plus.
-  introv Hlt Hyp. destruct l.
-  + easy.
-  + cbn in *. lia.
+  - simplify.
+    fsetdec.
 Qed.
 
 Theorem lc_lam : forall (L : AtomSet.t) (t : term LN) (X : typ),
-    (forall x : atom, ~ x ∈@ L -> locally_closed (t '(tvar (Fr x)))) ->
-    locally_closed (λ X t).
+    (forall x : atom, ~ x `in` L -> LC (t '(x: term LN))) ->
+    LC (λ X t).
 Proof.
-  introv hyp1. unfold locally_closed in *.
-  rewrite term_lc_gap2. specialize_freshly hyp1.
-  rewrite (open_lc_gap_eq_var_1). eauto.
+  introv HLC.
+  simplify_LC.
+  specialize_freshly HLC.
+  change (fvar e) with (ret (Fr e)) in HLC.
+  rewrite <- open_var_lcn_1 in HLC.
+  assumption.
 Qed.
 
-Theorem j_lc : forall Γ t A,
-    Γ ⊢ t : A -> locally_closed t.
+Theorem j_lc : forall Γ t τ,
+    Γ ⊢ t : τ -> LC t.
 Proof.
-  introv J. induction J.
-  - now rewrite term_lc12.
-  - pick fresh y excluding L and apply lc_lam; auto.
-  - now rewrite term_lc3.
+  introv J. typing_induction.
+  - simplify_LN. exact I.
+  - pick fresh y excluding L and apply lc_lam.
+    apply IHbody; auto.
+  - simplify_LN. split; assumption.
 Qed.
 
-Theorem weakening : forall Γ1 Γ2 Γ' (t : term LN) (A : typ),
+Theorem weakening : forall Γ1 Γ2 Γ' (t : term LN) (τ: typ),
     uniq Γ' ->
     disjoint Γ' (Γ1 ++ Γ2) ->
-    (Γ1 ++ Γ2 ⊢ t : A) ->
-    (Γ1 ++ Γ' ++ Γ2 ⊢ t : A).
+    (Γ1 ++ Γ2 ⊢ t : τ) ->
+    (Γ1 ++ Γ' ++ Γ2 ⊢ t : τ).
 Proof.
   introv Huq Hdj J.
   remember (Γ1 ++ Γ2) as Γrem.
   generalize dependent Γ2.
-  induction J; intros; subst.
-  - apply j_var. autorewrite with tea_rw_uniq tea_rw_disj in *.
-    rewrite disjoint_sym. preprocess. intuition.
-    simpl_list in *. intuition.
-  - rename H0 into IH. pick fresh y and apply j_abs.
-    specialize_cof IH y. simpl_alist in *.
-    apply IH; auto. autorewrite with tea_rw_disj in *.
-    splits; try easy. fsetdec.
+  typing_induction; intros Γ2 HeqΓ; subst.
+  - apply j_var.
+    { autorewrite with tea_rw_uniq tea_rw_disj in *.
+      rewrite disjoint_sym.
+      preprocess; intuition. }
+    simpl_list in *.
+    intuition.
+  - pick fresh y and apply j_abs.
+    specialize_cof IHbody y.
+    simpl_alist in IHbody.
+    simpl_alist.
+    apply IHbody.
+    { autorewrite with tea_rw_disj in *.
+      splits; try easy. fsetdec. }
+    { reflexivity. }
   - eauto using j_app.
 Qed.
 
-Corollary weakening_r : forall Γ1 (t : term LN) (A : typ),
-    (Γ1 ⊢ t : A) ->
-    forall Γ2, uniq Γ2 -> disjoint Γ1 Γ2 -> Γ1 ++ Γ2 ⊢ t : A.
+Corollary weakening_r : forall Γ1 (t : term LN) (τ: typ),
+    (Γ1 ⊢ t : τ) ->
+    forall Γ2, uniq Γ2 -> disjoint Γ1 Γ2 -> Γ1 ++ Γ2 ⊢ t : τ.
 Proof.
   intros.
   rewrite <- (List.app_nil_r Γ1) in H.
   rewrite <- (List.app_nil_r (Γ1 ++ Γ2)).
   rewrite <- List.app_assoc.
-  apply weakening; auto. List.simpl_list.
+  apply weakening; auto.
+  List.simpl_list.
   eauto with tea_alist.
 Qed.
 
-Theorem substitution : forall Γ1 Γ2 (x : atom) (t u : term LN) (A B : typ),
-    (Γ1 ++ x ~ A ++ Γ2 ⊢ t : B) ->
-    (Γ1 ⊢ u : A) ->
-    (Γ1 ++ Γ2 ⊢ t '{x ~> u} : B).
+Theorem substitution: forall Γ1 Γ2 x t u τ1 τ2,
+    (Γ1 ++ x ~ τ1 ++ Γ2 ⊢ t : τ2) ->
+    (Γ1 ⊢ u : τ1) ->
+    Γ1 ++ Γ2 ⊢ t '{x ~> u} : τ2.
 Proof.
   introv Jt Ju.
-  specialize (j_ctx_wf (Γ1 ++ x~A ++ Γ2)); intro Hwf.
-  assert (locally_closed u) by (eauto using j_lc).
-  remember (Γ1 ++ x ~ A ++ Γ2) as Γrem. generalize dependent Γ2.
-  induction Jt; intros.
-  - cbn. compare values x and x0.
-    + assert (A0 = A) by eauto using binds_mid_eq; subst.
-      autorewrite with tea_rw_uniq tea_rw_disj in *.
+  specialize (j_ctx_wf (Γ1 ++ x ~ τ1 ++ Γ2)); intro Hwf.
+  assert (LC u) by (eauto using j_lc).
+  remember (Γ1 ++ x ~ τ1 ++ Γ2) as Γrem.
+  generalize dependent Γ2.
+  typing_induction_on Jt; intros Γ2 HeqΓ.
+  - compare values x and x0.
+    + simplify_subst.
+      simpl_local.
+      assert (τ = τ1) by eauto using binds_mid_eq; subst.
       apply weakening_r.
-      * easy.
-      * easy.
-      * intuition (auto with tea_alist).
-    + constructor; eauto using uniq_remove_mid, binds_remove_mid.
-  - cbn. apply j_abs with (L := L ∪ domset Γ ∪ {{x}}).
-    intros_cof H1.
-    unfold preincr. reassociate ->. rewrite (extract_incr).
-    change (binddt (subst_loc x u ∘ extract) t)
-      with (t '{x ~> u}).
-    change (@tvar) with (@ret term _).
+      { assumption. }
+      { autorewrite with tea_rw_uniq tea_rw_disj in *.
+        intuition. }
+      { autorewrite with tea_rw_uniq tea_rw_disj in *.
+        intuition. }
+    + simplify_subst.
+      simpl_local.
+      apply j_var.
+      { autorewrite with tea_rw_uniq tea_rw_disj in *.
+        intuition. }
+      { eauto using binds_remove_mid. }
+  - simplify_subst.
+    apply j_abs with (L := L ∪ domset Γ ∪ {{x}}).
+    intros_cof IHbody.
+    change (fvar e) with (ret (Fr e)).
     rewrite <- subst_open_var.
-    + simpl_alist in *. eapply H1.
+    + simpl_alist in *.
+      eapply IHbody.
       * eauto using j_ctx_wf.
       * subst. now simpl_alist.
     + fsetdec.
     + auto.
-  - cbn. eauto using j_app.
+  - simplify. eauto using j_app.
 Qed.
 
 Corollary substitution_r : forall Γ (x : atom) (t u : term LN) (A B : typ),
@@ -204,48 +217,47 @@ Inductive value : term LN -> Prop :=
 Inductive beta_step : term LN -> term LN -> Prop :=
 | beta_app_l : forall (t1 t2 t1' : term LN),
     beta_step t1 t1' ->
-    beta_step ([t1]@[t2]) ([t1']@[t2])
+    beta_step (⟨t1⟩ (t2)) (⟨t1'⟩(t2))
 | beta_app_r : forall (t1 t2 t2' : term LN),
     beta_step t2 t2' ->
-    beta_step ([t1]@[t2]) ([t1]@[t2'])
-| beta_beta : forall (X : typ) (t u : term LN),
-    beta_step ([λ X t]@[u]) (t '(u)).
+    beta_step (⟨t1⟩(t2)) (⟨t1⟩(t2'))
+| beta_beta : forall τ t u,
+    beta_step (⟨λ τ t⟩(u)) (t '(u)).
 
 Theorem subject_reduction_step : forall (t t' : term LN) Γ A,
     Γ ⊢ t : A -> beta_step t t' -> Γ ⊢ t' : A.
 Proof.
-  intros t t' Γ A J step.
+  introv J Hstep.
   generalize dependent t'.
-  induction J.
-  - intros; inversion step.
-  - intros; inversion step.
-  - intros; inversion step.
-    + subst. apply j_app with (A := A); auto.
-    + subst. apply j_app with (A := A); auto.
-    + subst. apply inversion21 in J1.
+  typing_induction; intros t' Hstep.
+  - inversion Hstep.
+  - inversion Hstep.
+  - inversion Hstep.
+    + subst. eauto using j_app.
+    + subst. eauto using j_app.
+    + subst.
+      apply inversion21 in J1.
       destruct J1 as [C [hyp1 [L hyp2]]].
       inversion hyp1; subst.
       specialize_freshly hyp2.
-      assert (rw : t '(t2) = t '(tvar (Fr e)) '{e ~> t2}).
-      { erewrite open_spec_eq. reflexivity.
-        fsetdec. }
-      rewrite rw. eapply substitution_r.
-      exact hyp2. assumption.
+      rewrite (open_spec _ _ e).
+      { eauto using substitution_r. }
+      { fsetdec. }
 Qed.
 
-Theorem progress : forall (t : term LN) A,
-    nil ⊢ t : A -> value t \/ (exists t', beta_step t t').
+Theorem progress : forall (t : term LN) τ1,
+    nil ⊢ t : τ1 -> value t \/ (exists t', beta_step t t').
 Proof.
-  intros. remember [] as ctx.
-  induction H.
-  - subst. inversion H0.
-  - left; constructor.
-  - rename IHJudgment1 into IH1.
-    rename IHJudgment2 into IH2.
-    specialize (IH1 Heqctx); specialize (IH2 Heqctx).
-    destruct IH1.
-    + inversion H1; subst.
-      right. exists (t '(t2)). constructor.
-    + right. destruct H1. eexists.
-      apply beta_app_l. eauto.
+  introv J. remember [] as ctx.
+  typing_induction; subst.
+  - inversion Hin.
+  - left. constructor.
+  - specialize (IHJ1 eq_refl).
+    specialize (IHJ2 eq_refl).
+    destruct IHJ1.
+    + right. inversion H; subst.
+      exists (t '(t2)). constructor.
+    + right.
+      destruct H as [t1' Hstep'].
+      eauto using beta_app_l.
 Qed.
